tidy

isabelle/CVM_Original/Algo.thy
@@ -45,8 +45,8 @@ abbreviation
 text
   \<open>The algorithm is defined in the SPMF monad (with None representing failure)\<close>
 
-definition step :: \<open>'a \<Rightarrow> 'a state \<Rightarrow> 'a state spmf\<close> where
-  \<open>step \<equiv> \<lambda> x state. do {
+definition step_1 :: \<open>'a \<Rightarrow> 'a state \<Rightarrow> 'a state spmf\<close> where
+  \<open>step_1 \<equiv> \<lambda> x state. do {
     let k = state_k state;
     let chi = state_chi state;
 
@@ -57,17 +57,27 @@ definition step :: \<open>'a \<Rightarrow> 'a state \<Rightarrow> 'a state spmf\
       then insert x
       else Set.remove x);
 
-    if card chi < threshold
-    then return_spmf (state\<lparr>state_chi := chi\<rparr>)
-    else do {
-      keep_in_chi :: 'a \<Rightarrow> bool \<leftarrow> prod_pmf chi \<lblot>bernoulli_pmf f\<rblot>;
+    return_spmf (state\<lparr>state_chi := chi\<rparr>) }\<close>
 
-      let chi = Set.filter keep_in_chi chi;
-      let k = k + 1;
+definition step_2 :: \<open>'a state \<Rightarrow> 'a state spmf\<close> where
+  \<open>step_2 \<equiv> \<lambda> state.
+    let
+      k = state_k state;
+      chi = state_chi state
+    in if card chi < threshold
+      then return_spmf (state\<lparr>state_chi := chi\<rparr>)
+      else do {
+        keep_in_chi :: 'a \<Rightarrow> bool \<leftarrow> prod_pmf chi \<lblot>bernoulli_pmf f\<rblot>;
 
-      if card chi < threshold
-      then return_spmf \<lparr>state_k = k, state_chi = chi\<rparr>
-      else fail_spmf }}\<close>
+        let chi = Set.filter keep_in_chi chi;
+        let k = k + 1;
+
+        if card chi < threshold
+        then return_spmf \<lparr>state_k = k, state_chi = chi\<rparr>
+        else fail_spmf }\<close>
+
+definition step :: \<open>'a \<Rightarrow> 'a state \<Rightarrow> 'a state spmf\<close> where
+  \<open>step \<equiv> \<lambda> x. step_1 x >=> step_2\<close>
 
 abbreviation
   \<open>run_steps_then_estimate_spmf \<equiv>
